heap_lang/heap.v
@@ -130,7 +130,7 @@ Section heap.
 
   (** Weakest precondition *)
   Lemma wp_alloc E e v :
-    to_val e = Some v → nclose heapN ⊆ E →
+    to_val e = Some v → ↑heapN ⊆ E →
     {{{ heap_ctx }}} Alloc e @ E {{{ l, RET LitV (LitLoc l); l ↦ v }}}.
   Proof.
     iIntros (<-%of_to_val ? Φ) "#Hinv HΦ". rewrite /heap_ctx.
@@ -144,7 +144,7 @@ Section heap.
   Qed.
 
   Lemma wp_load E l q v :
-    nclose heapN ⊆ E →
+    ↑heapN ⊆ E →
     {{{ heap_ctx ∗ ▷ l ↦{q} v }}} Load (Lit (LitLoc l)) @ E
     {{{ RET v; l ↦{q} v }}}.
   Proof.
@@ -157,7 +157,7 @@ Section heap.
   Qed.
 
   Lemma wp_store E l v' e v :
-    to_val e = Some v → nclose heapN ⊆ E →
+    to_val e = Some v → ↑heapN ⊆ E →
     {{{ heap_ctx ∗ ▷ l ↦ v' }}} Store (Lit (LitLoc l)) e @ E
     {{{ RET LitV LitUnit; l ↦ v }}}.
   Proof.
@@ -173,7 +173,7 @@ Section heap.
   Qed.
 
   Lemma wp_cas_fail E l q v' e1 v1 e2 v2 :
-    to_val e1 = Some v1 → to_val e2 = Some v2 → v' ≠ v1 → nclose heapN ⊆ E →
+    to_val e1 = Some v1 → to_val e2 = Some v2 → v' ≠ v1 → ↑heapN ⊆ E →
     {{{ heap_ctx ∗ ▷ l ↦{q} v' }}} CAS (Lit (LitLoc l)) e1 e2 @ E
     {{{ RET LitV (LitBool false); l ↦{q} v' }}}.
   Proof.
@@ -186,7 +186,7 @@ Section heap.
   Qed.
 
   Lemma wp_cas_suc E l e1 v1 e2 v2 :
-    to_val e1 = Some v1 → to_val e2 = Some v2 → nclose heapN ⊆ E →
+    to_val e1 = Some v1 → to_val e2 = Some v2 → ↑heapN ⊆ E →
     {{{ heap_ctx ∗ ▷ l ↦ v1 }}} CAS (Lit (LitLoc l)) e1 e2 @ E
     {{{ RET LitV (LitBool true); l ↦ v2 }}}.
   Proof.
